Kroopt/Core/RecordPath.lean
@@ -231,7 +231,8 @@ def handleCryptoResultCorrelated (s : State) (op : OperationId) (r : CryptoResul
       recordFailAlert s .badRecordMac (.crypto .authFailed)
   | .failed e =>
       recordFailAlert s .internalError (.crypto e)
-  | .randomBytes _ => .ok (s.clearOp op, [])
+  | .randomBytes b => handshakeOnGatingResult s op (.randomBytes b)
+  | .finishedMac vd => handshakeOnGatingResult s op (.finishedMac vd)
   | .ecdheComplete srv h => handshakeOnGatingResult s op (.ecdheComplete srv h)
   | .hkdfSecret d => handshakeOnGatingResult s op (.hkdfSecret d)
   | .keysInstalled => handshakeOnGatingResult s op .keysInstalled
